{
 "cells": [
  {
   "cell_type": "code",
   "execution_count": null,
   "metadata": {
    "collapsed": true
   },
   "outputs": [],
   "source": [
    "-- http://courses.cms.caltech.edu/cs11/material/haskell/\n",
    "-- Lab 3\n",
    "\n",
    "data AbstractInteger = Zero | Succ AbstractInteger | Pred AbstractInteger\n",
    "                         deriving(Show, Eq)\n",
    "                         \n",
    "instance Ord AbstractInteger where\n",
    "  \n",
    "  compare (Pred x) (Pred y) = compare x y \n",
    "  compare (Pred _) Zero = LT\n",
    "  compare (Pred _) (Succ _) = LT\n",
    "  compare (Succ _) (Pred _) = GT\n",
    "  compare (Succ _) Zero = GT\n",
    "  compare (Succ x) (Succ y)  = compare x y \n",
    "  compare Zero (Pred _) = GT \n",
    "  compare Zero Zero = EQ \n",
    "  compare Zero (Succ _) = LT\n",
    "  \n",
    "  x < y = compare x y == LT\n",
    "  x <= y = compare x y /= GT\n",
    "  x > y = compare x y == GT\n",
    "  x >= y = compare x y /= LT\n",
    "  max x y = if x < y then y else x\n",
    "  min x y = if x < y then x else y\n",
    "  \n",
    "instance Num AbstractInteger where\n",
    "  \n",
    "  plus Zero \n",
    "  a + Zero = a\n",
    "  Zero + a = a\n",
    "  Zero + Zero = Zero\n",
    "  (Pred x) + (Succ y) = x + y\n",
    "  (Succ x) + (Pred y) = x + y\n",
    "  x0@(Succ _) + (Succ y) = (Succ x0) + y\n",
    "  x0@(Pred _) + (Pred y) = (Pred x0) + y\n",
    "  \n",
    "  x - y = x + (negate y)\n",
    "  \n",
    "  x@(Pred _) * y@(Pred _) = negate x * negate y\n",
    "  x@(Pred _) * y@(Succ _) = negate $ negate x * y \n",
    "  x@(Succ _) * y@(Pred _) = y * x \n",
    "  x@(Succ _) * y@(Succ _) = x + x * (y - (Succ Zero))\n",
    "  _ * Zero = Zero\n",
    "  Zero * _ = Zero\n",
    "  \n",
    "  negate Zero = Zero\n",
    "  negate (Succ x) = Pred $ negate x\n",
    "  negate (Pred x) = Succ $ negate x\n",
    "  \n",
    "  abs x@(Pred _) = negate x\n",
    "  abs Zero = Zero\n",
    "  abs x@(Succ _) = x \n",
    "  \n",
    "  signum (Pred x) = negate x\n",
    "  signum (Succ x) = x\n",
    "  signum Zero = Zero\n",
    "  \n",
    "  fromInteger n \n",
    "    | n < 0 = Pred $ fromInteger (n + 1)\n",
    "    | n == 0 = Zero\n",
    "    | otherwise = Succ $ fromInteger (n - 1)\n",
    "  \n",
    "  \n",
    "ai_toInteger :: AbstractInteger -> Integer\n",
    "ai_toInteger Zero = 0\n",
    "ai_toInteger (Succ x) = 1 + ai_toInteger x\n",
    "ai_toInteger (Pred x) = (-1) + ai_toInteger x\n",
    "\n",
    "factorial :: (Num a, Ord a) => a -> a\n",
    "factorial x | x < fromInteger 0 = error \"x must be integral and nonnegative\"\n",
    "            | x == fromInteger 0 = fromInteger 1\n",
    "            | otherwise = x * factorial (x - fromInteger 1)\n",
    "\n",
    "factorialTR :: (Num a, Ord a) => a -> a\n",
    "factorialTR x = factTR x 1\n",
    "    where factTR x n | x < fromInteger 0 = error \"x must be integral and nonnegative\"\n",
    "                     | x == fromInteger 0 = n\n",
    "                     | otherwise = factTR (x - fromInteger 1) (x * n)\n",
    "  \n",
    "data Quaternion = Q Double Double Double Double\n",
    "                         deriving(Eq)\n",
    "                         \n",
    "instance Show Quaternion where\n",
    "\n",
    "    show (Q r i j k) = \"(\" ++ show r ++ \" + \" ++ show i ++ \"i + \" ++ show j ++ \"j + \" ++ show k ++ \"k\" ++ \")\"\n",
    "    \n",
    "instance Num Quaternion where\n",
    "\n",
    "    Q a0 b0 c0 d0 + (Q a1 b1 c1 d1) = Q (a0 + a1) (b0 + b1) (c0 + c1) (d0 + d1)\n",
    "    \n",
    "    Q a0 b0 c0 d0 - (Q a1 b1 c1 d1) = Q (a0 - a1) (b0 - b1) (c0 - c1) (d0 - d1)\n",
    "    \n",
    "    Q a1 b1 c1 d1 * (Q a2 b2 c2 d2) = Q (a1*a2 - b1*b2 - c1*c2 - d1*d2) (a1*b2 + b1*a2 + c1*d2 - d1*c2) (a1*c2 - b1*d2 + c1*a2 + d1*b2) (a1*d2 + b1*c2 - c1*b2 + d1*a2)\n",
    "    \n",
    "    negate (Q a b c d) = Q (-a) (-b) (-c) (-d)\n",
    "    \n",
    "    abs (Q a b c d) = Q (sqrt (a*a + b*b + c*c + d*d)) 0.0 0.0 0.0\n",
    "    \n",
    "    signum q@(Q a b c d) = Q (a / z) (b / z) (c / z) (d / z)\n",
    "                                    where Q z _ _ _ = abs q\n",
    "\n",
    "    fromInteger n = Q (fromInteger n) 0.0 0.0 0.0"
   ]
  }
 ],
 "metadata": {
  "kernelspec": {
   "display_name": "Haskell",
   "language": "haskell",
   "name": "haskell"
  },
  "language_info": {
   "codemirror_mode": "ihaskell",
   "file_extension": ".hs",
   "name": "haskell",
   "version": "7.10.3"
  }
 },
 "nbformat": 4,
 "nbformat_minor": 0
}
